lock_offset
I need to proove that I'm assigning a lock to my temp variable

progs/verif_bst_conc.v
@@ -94,7 +94,30 @@ Arguments delete {V} x s.
 
 Eval hnf in reptype (nested_field_type t_struct_tree_t [StructField _lock]).
 
+(*Definition t_lock_pred' tl lsh p lock  := EX t : tree val, t_lock_pred tl lsh t p lock.
 
+Definition t_lock_pred_uncurry (t: tree val) lsh (tl : (tree val -> (val * val) -> mpred)) := fun t '(p, lock) => 
+  t_lock_pred tl t lsh p lock.
+
+Definition t_lock_pred'' t lsh :=  HORec (t_lock_pred_uncurry t lsh).
+
+Definition t_lock_pred''' t lsh p lock  := t_lock_pred'' t lsh (p,lock).
+
+
+Definition ltree_final lsh p lock (t : tree val) :=
+  !!(field_compatible t_struct_tree_t nil p) &&
+  (field_at lsh t_struct_tree_t [StructField _lock] lock p *
+   lock_inv lsh lock (t_lock_pred''' t lsh p lock)).
+*)   
+
+Fixpoint tree_rep (t: tree val) (p: val) : mpred := (*tree strored in p correctly, see struct tree, representation in memory*)
+ match t with
+ | E => !!(p=nullval) && emp
+ | T a x v b => !! (Int.min_signed <= x <= Int.max_signed /\ tc_val (tptr Tvoid) v) &&
+    EX pa:val, EX pb:val,
+    data_at Tsh t_struct_tree (Vint (Int.repr x),(v,(pa,pb))) p *
+    tree_rep a pa * tree_rep b pb
+ end.
 
 
 Definition ltree tl lsh p lock :=
@@ -116,21 +139,7 @@ EX tp : val, (data_at Tsh (tptr t_struct_tree) tp p * node_rep tl lsh t tp *
   malloc_token Tsh (t_struct_tree_t) p *
  malloc_token Tsh (tlock) lock).
 
-(*Definition t_lock_pred' tl lsh p lock  := EX t : tree val, t_lock_pred tl lsh t p lock.
 
-Definition t_lock_pred_uncurry (t: tree val) lsh (tl : (tree val -> (val * val) -> mpred)) := fun t '(p, lock) => 
-  t_lock_pred tl t lsh p lock.
-
-Definition t_lock_pred'' t lsh :=  HORec (t_lock_pred_uncurry t lsh).
-
-Definition t_lock_pred''' t lsh p lock  := t_lock_pred'' t lsh (p,lock).
-
-
-Definition ltree_final lsh p lock (t : tree val) :=
-  !!(field_compatible t_struct_tree_t nil p) &&
-  (field_at lsh t_struct_tree_t [StructField _lock] lock p *
-   lock_inv lsh lock (t_lock_pred''' t lsh p lock)).
-*)   
 Definition t_lock_pred' tl lsh p lock  := 
       EX t : tree val, t_lock_pred tl t lsh p lock.
 
@@ -156,15 +165,70 @@ Admitted.
    
 
 
-(*Definition treebox_rep (t: tree val) (b: val) :=
+Definition treebox_rep (t: tree val) (b: val) :=
  EX p: val, data_at Tsh (tptr t_struct_tree_t) p b.
- *)
+ 
  
 Definition nodebox_rep (sh : share) (lock : val) (nb: val) :=
  EX np: val, data_at Tsh (tptr (t_struct_tree_t)) np nb * ltree_final sh np lock.
  
+
+
+
+Definition mallocN_spec :=
+ DECLARE _mallocN
+  WITH n: Z
+  PRE [ 1%positive OF tint]
+     PROP (4 <= n <= Int.max_unsigned)
+     LOCAL (temp 1%positive (Vint (Int.repr n)))
+     SEP ()
+  POST [ tptr tvoid ]
+     EX v: val,
+     PROP (malloc_compatible n v)
+     LOCAL (temp ret_temp v)
+     SEP (memory_block Tsh n v).
+
+Definition freeN_spec :=
+ DECLARE _freeN
+  WITH p : val , n : Z
+  PRE [ 1%positive OF tptr tvoid , 2%positive OF tint]
+     (* we should also require natural_align_compatible (eval_id 1) *)
+      PROP() LOCAL (temp 1%positive p; temp 2%positive (Vint (Int.repr n)))
+      SEP (memory_block Tsh n p)
+  POST [ tvoid ]
+    PROP () LOCAL () SEP ().
+    
+    
+
+Definition treebox_new_spec :=
+ DECLARE _treebox_new
+  WITH u : unit
+  PRE  [  ]
+       PROP() LOCAL() SEP ()
+  POST [ tptr (tptr t_struct_tree) ]
+    EX v:val,
+    PROP()
+    LOCAL(temp ret_temp v)
+    SEP (data_at Tsh (tptr t_struct_tree) nullval v).
+
+(*Definition insert_spec :=
+ DECLARE _insert
+  WITH b: val, x: Z, v: val, t: tree val
+  PRE  [ _t OF (tptr (tptr t_struct_tree)), _x OF tint,
+        _value OF (tptr Tvoid)   ]
+    PROP( Int.min_signed <= x <= Int.max_signed; is_pointer_or_null v)
+    LOCAL(temp _t b; temp _x (Vint (Int.repr x)); temp _value v)
+    SEP (treebox_rep t b)
+  POST [ Tvoid ] 
+    PROP()
+    LOCAL()
+    SEP (treebox_rep (insert x v t) b).
+*)  
+    
 (*maybe I should add the treebox_rep in the ltree definition *)
-Definition insert_spec' :=
+(*NEW*)
+Definition insert_spec :=
+  DECLARE _insert
   WITH sh : share, p : val, lock : val,
        b: val, x: Z, v: val, t: tree val
   PRE [  _t OF (tptr (tptr t_struct_tree_t)), _x OF tint,
@@ -176,9 +240,336 @@ Definition insert_spec' :=
    PROP ()
    LOCAL ()
    SEP (nodebox_rep sh lock b).
-Definition insert_spec prog := DECLARE (ext_link_prog prog "insert") insert_spec'.    
+(*Definition insert_spec prog := DECLARE (ext_link_prog prog "insert") insert_spec'.*)    
+
+Definition lookup_spec :=
+ DECLARE _lookup
+  WITH b: val, x: Z, v: val, t: tree val
+  PRE  [ _t OF (tptr (tptr t_struct_tree)), _x OF tint  ]
+    PROP( Int.min_signed <= x <= Int.max_signed)
+    LOCAL(temp _t b; temp _x (Vint (Int.repr x)))
+    SEP (treebox_rep t b)
+  POST [ tptr Tvoid ]
+    PROP()
+    LOCAL(temp ret_temp (lookup nullval x t))
+    SEP (treebox_rep t b).
+
+Definition turn_left_spec :=
+ DECLARE _turn_left
+  WITH ta: tree val, x: Z, vx: val, tb: tree val, y: Z, vy: val, tc: tree val, b: val, l: val, pa: val, r: val
+  PRE  [ __l OF (tptr (tptr (Tstruct _tree noattr))),
+        _l OF (tptr (Tstruct _tree noattr)),
+        _r OF (tptr (Tstruct _tree noattr))]
+    PROP(Int.min_signed <= x <= Int.max_signed; is_pointer_or_null vx)
+    LOCAL(temp __l b; temp _l l; temp _r r)
+    SEP (data_at Tsh (tptr t_struct_tree) l b;
+         data_at Tsh t_struct_tree (Vint (Int.repr x), (vx, (pa, r))) l;
+         tree_rep ta pa;
+         tree_rep (T tb y vy tc) r)
+  POST [ Tvoid ] 
+    EX pc: val,
+    PROP(Int.min_signed <= y <= Int.max_signed; is_pointer_or_null vy)
+    LOCAL()
+    SEP (data_at Tsh (tptr t_struct_tree) r b;
+         data_at Tsh t_struct_tree (Vint (Int.repr y), (vy, (l, pc))) r;
+         tree_rep (T ta x vx tb) l;
+         tree_rep tc pc).
+
+Definition pushdown_left_spec :=
+ DECLARE _pushdown_left
+  WITH ta: tree val, x: Z, v: val, tb: tree val, b: val, p: val
+  PRE  [ _t OF (tptr (tptr (Tstruct _tree noattr)))]
+    PROP(Int.min_signed <= x <= Int.max_signed; tc_val (tptr Tvoid) v)
+    LOCAL(temp _t b)
+    SEP (data_at Tsh (tptr t_struct_tree) p b;
+         field_at Tsh t_struct_tree [StructField _key] (Vint (Int.repr x)) p;
+         field_at Tsh t_struct_tree [StructField _value] v p;
+         treebox_rep ta (field_address t_struct_tree [StructField _left] p);
+         treebox_rep tb (field_address t_struct_tree [StructField _right] p))
+  POST [ Tvoid ] 
+    PROP()
+    LOCAL()
+    SEP (treebox_rep (pushdown_left ta tb) b).
+
+Definition delete_spec :=
+ DECLARE _delete
+  WITH b: val, x: Z, t: tree val
+  PRE  [ _t OF (tptr (tptr t_struct_tree)), _x OF tint]
+    PROP( Int.min_signed <= x <= Int.max_signed)
+    LOCAL(temp _t b; temp _x (Vint (Int.repr x)))
+    SEP (treebox_rep t b)
+  POST [ Tvoid ] 
+    PROP()
+    LOCAL()
+    SEP (treebox_rep (delete x t) b).
+
+Definition tree_free_spec :=
+ DECLARE _tree_free
+  WITH t: tree val, p: val
+  PRE  [ _p OF (tptr t_struct_tree) ]
+       PROP() LOCAL(temp _p p) SEP (tree_rep t p)
+  POST [ Tvoid ]
+    PROP()
+    LOCAL()
+    SEP (emp).
+
+Definition treebox_free_spec :=
+ DECLARE _treebox_free
+  WITH t: tree val, b: val
+  PRE  [ _b OF (tptr (tptr t_struct_tree)) ]
+       PROP() LOCAL(temp _b b) SEP (treebox_rep t b)
+  POST [ Tvoid ]
+    PROP()
+    LOCAL()
+    SEP (emp).
+
+Definition Gprog : funspecs :=
+    ltac:(with_library prog [
+    mallocN_spec; freeN_spec; treebox_new_spec;
+    tree_free_spec; treebox_free_spec;
+    insert_spec; lookup_spec;
+    turn_left_spec; pushdown_left_spec; delete_spec
+  ]).
+
+Lemma tree_rep_saturate_local:
+   forall tl lsh t p, node_rep tl lsh t p |-- !! is_pointer_or_null p.
+Proof.
+destruct t; simpl; intros.
+entailer!.
+Intros pa pb locka lockb. entailer!.
+Qed.
+
+Hint Resolve tree_rep_saturate_local: saturate_local.
+
+Lemma tree_rep_valid_pointer:
+  forall tl lsh t p, node_rep tl lsh t p |-- valid_pointer p.
+Proof.
+intros.
+destruct t; simpl; normalize; auto with valid_pointer.
+Qed.
+Hint Resolve tree_rep_valid_pointer: valid_pointer.
+
+(*Lemma treebox_rep_saturate_local:
+   forall t b, treebox_rep t b |-- !! field_compatible (tptr t_struct_tree_t) [] b.
+Proof.
+intros.
+unfold treebox_rep.
+Intros p.
+entailer!.
+Qed.
+
+Hint Resolve treebox_rep_saturate_local: saturate_local.
+
+Definition insert_inv (b0: val) (t0: tree val) (x: Z) (v: val): environ -> mpred :=
+  EX b: val, EX t: tree val,
+  PROP()
+  LOCAL(temp _t b; temp _x (Vint (Int.repr x));   temp _value v)
+  SEP(treebox_rep t b;  (treebox_rep (insert x v t) b -* treebox_rep (insert x v t0) b0)). (* b0 which points to t0 which is the entire tree *)
+*)
+Definition insert_inv (b0: val) (t0: tree val) (x: Z) (v: val): environ -> mpred :=
+  EX b: val, EX lock: val, EX lsh: share,
+  PROP()
+  LOCAL(temp _t b; temp _x (Vint (Int.repr x));   temp _value v)
+  SEP(nodebox_rep lsh lock b).
 
 
+Lemma ramify_PPQQ {A: Type} {NA: NatDed A} {SA: SepLog A} {CA: ClassicalSep A}: forall P Q,
+  P |-- P * (Q -* Q).
+Proof.
+  intros. Check RAMIF_PLAIN.solve.
+  apply RAMIF_PLAIN.solve with emp.
+  + rewrite sepcon_emp. auto.
+  + rewrite emp_sepcon. auto.
+Qed.
+
+Lemma tree_rep_nullval: forall tl t lsh,
+  node_rep tl lsh t nullval |-- !! (t = E).
+Proof.
+  intros.
+  destruct t; [entailer! |].
+  simpl node_rep.
+  Intros pa pb locka lockb. entailer!.
+Qed.
+
+Hint Resolve tree_rep_nullval: saturate_local.
+
+(*Lemma treebox_rep_leaf: forall x p b (v: val),
+  is_pointer_or_null v ->
+  Int.min_signed <= x <= Int.max_signed ->
+  data_at Tsh t_struct_tree (Vint (Int.repr x), (v, (nullval, nullval))) p * data_at Tsh (tptr t_struct_tree) p b |-- treebox_rep (T E x v E) b.
+Proof.
+  intros.
+  unfold treebox_rep, tree_rep. Exists p nullval nullval. entailer!.
+Qed.
+
+Lemma bst_left_entail: forall (t1 t1' t2: tree val) k (v p1 p2 p b: val),
+  Int.min_signed <= k <= Int.max_signed ->
+  is_pointer_or_null v ->
+  data_at Tsh (tptr t_struct_tree) p b *
+  data_at Tsh t_struct_tree (Vint (Int.repr k), (v, (p1, p2))) p *
+  node_rep t1 p1 * node_rep t2 p2
+  |-- treebox_rep t1 (field_address t_struct_tree [StructField _left] p) *
+       (treebox_rep t1'
+         (field_address t_struct_tree [StructField _left] p) -*
+        treebox_rep (T t1' k v t2) b).
+        Print StructField.
+Proof.
+  intros.
+  unfold_data_at (data_at _ _ _ p). Check field_at_data_at.
+  rewrite (field_at_data_at _ t_struct_tree [StructField _left]).
+  unfold treebox_rep at 1. Exists p1. cancel.
+  Check wand_sepcon_adjoint.
+  rewrite <- wand_sepcon_adjoint.
+  clear p1.
+  unfold treebox_rep.
+  Exists p.
+  simpl.
+  Intros p1.
+  Exists p1 p2.
+  entailer!.
+  unfold_data_at (data_at _ _ _ p).
+  rewrite (field_at_data_at _ t_struct_tree [StructField _left]).
+  cancel.
+Qed.
+
+Lemma bst_right_entail: forall (t1 t2 t2': tree val) k (v p1 p2 p b: val),
+  Int.min_signed <= k <= Int.max_signed ->
+  is_pointer_or_null v ->
+  data_at Tsh (tptr t_struct_tree) p b *
+  data_at Tsh t_struct_tree (Vint (Int.repr k), (v, (p1, p2))) p *
+  node_rep t1 p1 * node_rep t2 p2
+  |-- treebox_rep t2 (field_address t_struct_tree [StructField _right] p) *
+       (treebox_rep t2'
+         (field_address t_struct_tree [StructField _right] p) -*
+        treebox_rep (T t1 k v t2') b).
+Proof.
+  intros.
+  unfold_data_at (data_at _ _ _ p).
+  rewrite (field_at_data_at _ t_struct_tree [StructField _right]).
+  unfold treebox_rep at 1. Exists p2. cancel.
+
+  rewrite <- wand_sepcon_adjoint.
+  clear p2.
+  unfold treebox_rep.
+  Exists p.
+  simpl.
+  Intros p2.
+  Exists p1 p2.
+  entailer!.
+  unfold_data_at (data_at _ _ _ p).
+  rewrite (field_at_data_at _ t_struct_tree [StructField _right]).
+  cancel.
+Qed.
+*)
+Lemma modus_ponens_wand' {A}{ND: NatDed A}{SL: SepLog A}:
+  forall P Q R: A, P |-- Q -> P * (Q -* R) |-- R.
+Proof.
+  intros.
+  eapply derives_trans; [| apply modus_ponens_wand].
+  apply sepcon_derives; [| apply derives_refl].
+  auto.
+Qed.
+
+Lemma if_trueb: forall {A: Type} b (a1 a2: A), b = true -> (if b then a1 else a2) = a1.
+Proof. intros; subst; auto. Qed.
+
+Lemma if_falseb: forall {A: Type} b (a1 a2: A), b = false -> (if b then a1 else a2) = a2.
+Proof. intros; subst; auto. Qed.
+
+Ltac simpl_compb := first [ rewrite if_trueb by (apply Z.ltb_lt; omega)
+                          | rewrite if_falseb by (apply Z.ltb_ge; omega)].
+
+Lemma body_insert: semax_body Vprog Gprog f_insert insert_spec.
+Proof.
+  start_function.  Check semax_pre. Check semax_loop.
+  eapply semax_pre; [ (* what's semax_loop?*) 
+    | apply (semax_loop _ (insert_inv b t x v) (insert_inv b t x v) )]. (*P' = insert_inv b t x v *)
+  * (* Precondition *)
+    unfold insert_inv. 
+    Exists b lock sh. entailer. Check ramify_PPQQ.
+  * (* Loop body *)
+    unfold insert_inv.
+    Intros b1 lock1 sh1.
+    forward. (* Sskip *)
+    unfold nodebox_rep at 1. Intros p1.
+    forward. (* tgt=*t; *)
+      unfold ltree_final. entailer!.
+    unfold ltree_final.  
+    assert_PROP
+    (offset_val 4 p1 = field_address (tlock) [StructField _lock] p1).
+      1: entailer!. hint. rewrite field_address_offset.
+        hint. autorewrite with norm.  (* l=tgt->lock *)
+    forward_if.
+    + (* then clause *)
+      subst p1.
+      Time forward_call (sizeof t_struct_tree).
+        1: simpl. rep_omega.
+      Intros p'. Check memory_block_data_at_.
+      rewrite memory_block_data_at_ by auto.
+      forward. (* p->key=x; *)
+      simpl.
+      forward. (* p->value=value; *)
+      forward. (* p->left=NULL; *)
+      forward. (* p->right=NULL; *)
+      assert_PROP (t1= (@E _)).
+        1: entailer!.
+      subst t1. simpl tree_rep. Check prop_true_andp.
+      rewrite prop_true_andp by auto.
+      forward. (* *t = p; *)
+      forward. (* return; *)
+      Check modus_ponens_wand'.
+      apply modus_ponens_wand'. 
+      apply treebox_rep_leaf. auto. auto.
+    + (* else clause *)
+      destruct t1.
+        { simpl tree_rep. normalize. (*???*)}
+      simpl tree_rep.
+      Intros pa pb. clear H1.
+      forward. (* y=p->key; *)
+      forward_if; [ | forward_if ].
+      - (* Inner if, then clause: x<k *)
+        forward. (* t=&p->left *)
+        unfold insert_inv.
+        Exists (offset_val 8 p1) t1_1. (*why offset 8*)
+        entailer!. simpl. Print simpl_compb.
+        simpl_compb. 
+        (* TODO: SIMPLY THIS LINE *)
+        Print field_compatible. (*???*)
+        replace (offset_val 8 p1)
+          with (field_address t_struct_tree [StructField _left] p1)
+          by (unfold field_address; simpl;
+              rewrite if_true by auto with field_compatible; auto).
+        Check RAMIF_PLAIN.trans'.
+        apply RAMIF_PLAIN.trans'.
+        apply bst_left_entail. auto. auto.
+      - (* Inner if, second branch:  k<x *)
+        forward. (* t=&p->right *)
+        unfold insert_inv.
+        Exists (offset_val 12 p1) t1_2.
+        entailer!. simpl.
+        simpl_compb. simpl_compb. (*boolean comparison*)
+        (* TODO: SIMPLY THIS LINE *)
+        replace (offset_val 12 p1)
+          with (field_address t_struct_tree [StructField _right] p1)
+          by (unfold field_address; simpl;
+              rewrite if_true by auto with field_compatible; auto).
+        apply RAMIF_PLAIN.trans'.
+        apply bst_right_entail; auto.
+      - (* Inner if, third branch: x=k *)
+        assert (x=k) by omega.
+        subst x.  clear H H1 H3.
+        forward. (* p->value=value *)
+        forward. (* return *) simpl.
+        (* TODO: SIMPLY THIS LINE *)
+        simpl_compb.
+        simpl_compb.
+        apply modus_ponens_wand'.
+        unfold treebox_rep. Exists p1.
+        simpl tree_rep. Exists pa pb. entailer!.
+  * (* After the loop *)
+    forward.
+    unfold loop2_ret_assert. apply andp_left2. normalize. 
+Qed.
 
 
 
